Steel.CondSolver: generate shape

experiment/Experiment.Steel.CondSolver.fsti
@@ -11,6 +11,59 @@ open FStar.Tactics
 open Learn.Tactics.Util
 open FStar.Mul
 
+
+#set-options "--fuel 1 --ifuel 1"
+
+type cs_failure_goal_shape =
+  | GShape_truth_refl_list
+  | GShape_tree_cond
+
+noeq
+type cs_failure_enum =
+  | Fail_goal_shape : (expected : cs_failure_goal_shape) -> (goal : typ) -> cs_failure_enum
+  | Fail_post_unification
+  | Fail_cond_sol
+  | Fail_shape_unification : nat -> nat -> cs_failure_enum
+
+noeq
+type cs_failure_t = {
+  fail_enum    : cs_failure_enum;
+  original_exn : option exn
+}
+
+exception CSFailure of cs_failure_t
+
+let cs_failure_to_string (f : cs_failure_t) : Tac string =
+  let enum = f.fail_enum in
+  let msg = term_to_string (quote enum) in
+  match f.original_exn with
+  | None -> msg
+  | Some (TacticFailure o_msg) -> msg^"\noriginal failure: "^o_msg
+  | Some o_exn -> msg^"\noriginal exception: "^term_to_string (quote o_exn)
+
+
+// The following utilities are hacked to raise a failure at the location where they are called
+// FIXME? raise a CSFailure exception with a meaningful location
+private unfold
+let cs_try (#a : Type) (f : unit -> Tac a)
+           (fail_f : (cs_failure_enum -> Tac string) ->
+                     TacH a (requires fun _ -> True) (ensures fun _ r -> Tactics.Result.Failed? r))
+  : Tac a
+  = try f ()
+    with | e -> fail_f (fun ety -> let failure = {fail_enum = ety; original_exn = Some e} in
+                               cs_failure_to_string failure)
+
+private unfold
+let cs_raise (#a : Type)
+             (fail_f : (cs_failure_enum -> Tac string) ->
+                       TacH a (requires fun _ -> True) (ensures fun _ r -> Tactics.Result.Failed? r))
+  : TacH a (requires fun _ -> True) (ensures fun _ r -> Tactics.Result.Failed? r)
+  = fail_f (fun ety -> let failure = {fail_enum = ety; original_exn = None} in
+                    cs_failure_to_string failure)
+
+
+irreducible let __cond_solver__ : unit = ()
+
 (***** [truth_refl] *)
 
 noeq
@@ -65,17 +118,15 @@ let mk_truth_refl_list_goal () : Tac (list bool) =
     try (apply (`ReflLNil); None)
     with | _ -> try (apply (`ReflLTrue); Some true)
     with | _ -> try (apply (`ReflLFalse); Some false)
-    with | _ -> fail "mk_truth_refl_list")
+    with | _ -> cs_raise (fun f -> fail (f (Fail_goal_shape GShape_truth_refl_list (cur_goal ())))))
 
 let mk_truth_refl_list (ps : term) : Tac (list bool & term & binder) =
   let bs = fresh_uvar (Some (`(list bool))) in
   let bd, res = build (`truth_refl_list (`#ps) (`#bs)) mk_truth_refl_list_goal
   in res, bs, bd
 
-(*let _ =
-  assert True
-    by (let bs,_,_ = mk_truth_refl_list (`[(1 == 1); (1 == 2); (2 + 2 == 4)]) in
-        fail (term_to_string (quote bs)))*)
+(*let _ = assert True by (let bs,_,_ = mk_truth_refl_list (`[(1 == 1);
+  (1 == 2); (2 + 2 == 4)]) in fail (term_to_string (quote bs)))*)
 
 
 (*** Building an injection *)
@@ -94,6 +145,8 @@ let injective_on_domI (#a #b : Type) (f : a -> option b)
   : Lemma (injective_on_dom f)
   = FStar.Classical.forall_intro_2 (FStar.Classical.move_requires_2 prf)
 
+
+[@@ __cond_solver__]
 let rec build_injection_find (#trg_n : nat) (g mask : vec trg_n bool) (i : nat)
   : Tot (option (Fin.fin (i + trg_n))) (decreases trg_n)
   = match g, mask with
@@ -101,6 +154,7 @@ let rec build_injection_find (#trg_n : nat) (g mask : vec trg_n bool) (i : nat)
   | true :: _, true :: _ -> Some i
   | _ :: g,    _ :: mask -> build_injection_find #(trg_n-1) g mask (i+1)
 
+[@@ __cond_solver__]
 let rec build_injection_iter (#src_n #trg_n : nat) (g : ograph src_n trg_n) (mask : vec trg_n bool)
   : Tot (vec src_n (option (Fin.fin trg_n))) (decreases src_n)
   = match g with
@@ -111,6 +165,7 @@ let rec build_injection_iter (#src_n #trg_n : nat) (g : ograph src_n trg_n) (mas
                          | None   -> mask
              in y :: build_injection_iter #(src_n-1) g mask'
 
+[@@ __cond_solver__]
 let build_injection (#src_n #trg_n : nat) (g : ograph src_n trg_n)
   : Tot (vec src_n (option (Fin.fin trg_n)))
   = build_injection_iter g (Ll.initi 0 trg_n (fun _ -> true))
@@ -146,6 +201,7 @@ type partial_injection (#a : Type) (src trg : list a) =
   }
 
 
+[@@ __cond_solver__]
 let list_of_equalities (#a : Type) (src trg : list a) : list prop =
   L.flatten (L.map (fun x -> L.map #_ #prop (fun y -> (x == y)) trg) src)
 
@@ -158,6 +214,7 @@ val list_of_equalities_index (#a : Type) (src trg : list a) (i : Fin.fin (len sr
            L.index (list_of_equalities src trg) (i * len trg + j) == (L.index src i == L.index trg j))
 
 
+[@@ __cond_solver__]
 let rec list_to_matrix (#a : Type) (n0 n1 : nat) (l : vec (n0 * n1) a)
   : Tot (vec n0 (vec n1 a)) (decreases n0)
   = if n0 = 0 then []
@@ -171,6 +228,7 @@ val list_to_matrix_index (#a : Type) (n0 n1 : nat) (l : vec (n0 * n1) a) (i : Fi
           [SMTPat (L.index (L.index (list_to_matrix n0 n1 l) i) j)]
 
 
+[@@ __cond_solver__]
 let ograph_of_equalities (#a : Type) (src trg : list a) (bs : list bool)
       (rfl : truth_refl_list (list_of_equalities src trg) bs)
   : ograph (len src) (len trg)
@@ -185,6 +243,7 @@ val ograph_of_equalities_index (#a : Type) (src trg : list a) (bs : list bool)
           (ensures  L.index src i == L.index trg j)
 
 
+[@@ __cond_solver__]
 let build_partial_injection (#a : Type) (src trg : list a) (bs : list bool)
       (rfl : truth_refl_list (list_of_equalities src trg) bs)
   : partial_injection src trg
@@ -236,6 +295,7 @@ let _ = assert (U.print_util test_inj)
 let mask_len (mask : list bool) : nat =
   L.count true mask
 
+[@@ __cond_solver__]
 let rec filter_mask (#a : Type) (#len : nat) (mask : vec len bool) (l : vec len a)
   : Tot (vec (mask_len mask) a) (decreases l)
   = match mask, l with
@@ -243,6 +303,7 @@ let rec filter_mask (#a : Type) (#len : nat) (mask : vec len bool) (l : vec len 
   | true  :: mask, x :: xs -> x :: filter_mask #a #(len-1) mask xs
   | false :: mask, _ :: xs -> filter_mask #a #(len-1) mask xs
 
+[@@ __cond_solver__]
 let rec mask_push (#len : nat) (mask : vec len bool) (i : Fin.fin len {L.index mask i})
   : Tot (Fin.fin (mask_len mask))
   =
@@ -251,6 +312,7 @@ let rec mask_push (#len : nat) (mask : vec len bool) (i : Fin.fin len {L.index m
          if b then 1 + mask_push #(len-1) mask (i-1)
          else mask_push #(len-1) mask (i - 1)
 
+[@@ __cond_solver__]
 let rec mask_pull (#len : nat) (mask : vec len bool) (j : Fin.fin (mask_len mask))
   : Tot (i : Fin.fin len {L.index mask i}) (decreases mask)
   = match mask with
@@ -258,6 +320,7 @@ let rec mask_pull (#len : nat) (mask : vec len bool) (j : Fin.fin (mask_len mask
   | false :: mask -> 1 + mask_pull #(len - 1) mask j
 
 (* TODO? optimize *)
+[@@ __cond_solver__]
 let rec merge_fun_on_mask (#src_n : nat) (mask : vec src_n bool) (#b : Type)
       (f : (i : Fin.fin src_n {L.index mask i}) -> (j : Fin.fin (mask_len mask)) -> b)
       (g : (i : Fin.fin src_n {not (L.index mask i)}) -> b)
@@ -291,9 +354,11 @@ val filter_mask_push (#len : nat) (mask : vec len bool) (i : Fin.fin len {L.inde
 
 /// Masks to select the elements that have *not* been matched
 
+[@@ __cond_solver__]
 let ij_src_mask (#src_n : nat) (#b : Type) (ij : vec src_n (option b)) : vec src_n bool
   = L.map None? ij
 
+[@@ __cond_solver__]
 let ij_trg_mask (#src_n #trg_n : nat) (ij : vec src_n (option (Fin.fin trg_n))) : vec trg_n bool
   = Ll.initi 0 trg_n (fun j -> not (L.mem (Some j) ij))
 
@@ -312,6 +377,7 @@ type cond_sol (#a : Type) : (all : bool) -> list a -> list a -> Type =
 
 // ALT? define with cond_sol_inj
 /// [cond_sol_unmatched sl] is the subset of indices of the target that have not been matched.
+[@@ __cond_solver__]
 let rec cond_sol_unmatched (#a : Type) (#all : bool) (#src #trg : list a) (sl : cond_sol all src trg)
   : Tot (list (Fin.fin (len trg))) (decreases sl)
   = match sl with
@@ -322,10 +388,12 @@ let rec cond_sol_unmatched (#a : Type) (#all : bool) (#src #trg : list a) (sl : 
                 let mask = ij_trg_mask ij      in
                 L.map #_ #(Fin.fin (len trg)) (mask_pull mask) um
 
+[@@ __cond_solver__]
 let cond_sol_unmatched_v (#a : Type) (#all : bool) (#src #trg : list a) (sl : cond_sol all src trg)
   : list a
   = L.map (L.index trg) (cond_sol_unmatched sl)
 
+[@@ __cond_solver__]
 let rec cond_sol_inj (#a : Type) (#all : bool) (#src #trg : list a) (sl : cond_sol all src trg)
   : Tot (vec (len src) (Fin.fin (len trg))) (decreases sl)
   = match sl with
@@ -339,6 +407,7 @@ let rec cond_sol_inj (#a : Type) (#all : bool) (#src #trg : list a) (sl : cond_s
                   (fun _ j -> mask_pull mask_trg (L.index inj' j))
                   (fun i   -> Some?.v (L.index ij i))
 
+[@@ __cond_solver__]
 let cond_sol_bij (#a : Type) (#all : bool) (#src #trg : list a) (sl : cond_sol all src trg)
   : Fin.fin (len src + len (cond_sol_unmatched sl)) -> Fin.fin (len trg)
   = 
@@ -373,12 +442,14 @@ val cond_sol_bij_spec (#a : Type) (#all : bool) (#src #trg : list a) (sl : cond_
            L.(src @ cond_sol_unmatched_v sl) == Perm.apply_perm_r (Perm.mk_perm_f (len trg) (cond_sol_bij sl)) trg)
 
 
+[@@ __cond_solver__]
 let cond_sol_to_equiv (#a : Type) (#all : bool) (#src #trg : list a) (sl : cond_sol all src trg)
   : Tot (Perm.pequiv trg L.(src @ cond_sol_unmatched_v sl))
   =
     (**) cond_sol_bij_spec sl;
     Perm.mk_perm_f (len trg) (cond_sol_bij sl)
 
+[@@ __cond_solver__]
 let cond_sol_all_to_equiv (#a : Type) (#src #trg : list a) (sl : cond_sol true src trg)
   : Tot (Perm.pequiv trg src)
   =
@@ -400,9 +471,9 @@ let build_cond_sol (all : bool) : Tac unit
       norm normal_build_partial_injection;
       norm normal_ij_mask;
     try if all then apply (`CSeq) else apply (`CSnil)
-    with | _ -> fail "build_cond_sol"
+    with | _ -> cs_raise (fun f -> fail (f Fail_cond_sol))
 
-// TODO
+
 let normal_cond_sol_to_equiv : list norm_step = [
     delta_only [`%cond_sol_to_equiv; `%cond_sol_bij; `%len; `%L.length; `%L.index];
     iota; zeta; primops
@@ -419,64 +490,41 @@ let _ = assert (U.print_util (cond_sol_to_equiv (test_cond_sol)))
 
 (*** Building [M.tree_cond] *)
 
-// TODO: comment; generate shape; exceptions
+/// The front-end tactic is [build_prog_cond], which solves a goal of the form [M.prog_cond t pre post] where
+/// [t], [pre] and [post] are concrete terms (i.e. do not contain uvars).
+/// Internally the main work is done by [build_tree_cond] which:
+/// - solves a goal of the form [M.prog_cond t pre post] where [t] and [pre] are concrete terms but
+///   [post] can be an uvar
+/// - returns the shape of the program as a [pre_shape_tree]
 
-open Steel.Effect.Common
 
-/// u : uvar
-/// p : post
+[@@ __cond_solver__]
+let serialize_perm (#n : nat) (f : Perm.perm_f n) : Perm.perm_f n
+  =
+    let l = Perm.perm_f_to_list f in
+    Perm.perm_f_of_list l
+
+let serialize_perm_id (#n : nat) (f : Perm.perm_f n)
+  : Lemma (serialize_perm f == f) [SMTPat (serialize_perm f)]
+  = Perm.perm_f_extensionality (serialize_perm f) f (fun i -> ())
 
 
-// TODO
+let normal_cond_solver : list norm_step = [
+    delta_only [`%len; `%None?; `%op_Negation; `%Some?.v;
+                `%L.append; `%L.flatten; `%L.hd; `%L.index; `%L.length; `%L.map; `%L.mem; `%L.op_At; `%L.splitAt;
+                `%L.tail; `%L.tl;
+                `%Ll.initi; `%Ll.set;
+                `%Perm.mk_perm_f; `%Perm.perm_f_to_list];
+    delta_attr [`%__tac_helper__; `%__cond_solver__];
+    delta_qualifier ["unfold"];
+    iota; zeta; primops
+  ]
+
 let norm_cond_sol () : Tac unit =
-  norm normal_build_partial_injection;
-  norm [delta_only [`%cond_sol_unmatched_v; `%cond_sol_unmatched;
-                    `%len; `%L.length; `%Ll.initi];
-        delta_qualifier ["unfold"];
-        iota; zeta; primops];
-  norm normal_ij_mask;
-  norm [delta_only [`%L.index; `%mask_pull; `%L.hd; `%L.tl; `%L.tail; `%L.op_At; `%L.append];
-        delta_qualifier ["unfold"];
-        iota; zeta; primops]
+  norm normal_cond_solver
 
-
-let __build_TCspec_u
-      (#a : Type) (#pre : M.pre_t) (#post : M.post_t a) (#req : M.req_t pre) (#ens : M.ens_t pre a post)
-      (#pre' : M.pre_t)
-      (cs0 : cond_sol false pre pre')
-  : M.tree_cond (M.Tspec a pre post req ens) pre' (fun (x : a) -> L.(post x @ cond_sol_unmatched_v cs0))
-  =
-    let frame = cond_sol_unmatched_v cs0 in
-    M.TCspec pre' (fun x -> L.(post x @ frame)) frame
-             (cond_sol_to_equiv cs0)
-             (fun x -> Perm.id_n (len L.(post x @ frame)))
-
-let __build_TCspec_p
-      (#a : Type) (#pre : M.pre_t) (#post : M.post_t a) (#req : M.req_t pre) (#ens : M.ens_t pre a post)
-      (#pre' : M.pre_t) (#post' : M.post_t a)
-      (cs0 : cond_sol false pre pre')
-      (cs1 : (x : a) -> cond_sol true (post' x) L.(post x @ cond_sol_unmatched_v cs0))
-  : M.tree_cond (M.Tspec a pre post req ens) pre' post'
-  =
-    M.TCspec pre' post' (cond_sol_unmatched_v cs0)
-             (cond_sol_to_equiv cs0) (fun x -> cond_sol_all_to_equiv (cs1 x))
-
-
-let __build_TCret_u
-      (#a : Type) (#x : a)
-      (#pre : M.pre_t)
-  : M.tree_cond (M.Tret a x) pre (fun _ -> pre)
-  =
-    M.TCret pre (fun _ -> pre) (Perm.id_n (len pre))
-
-let __build_TCret_p
-      (#a : Type) (#x : a)
-      (#pre : M.pre_t) (#post : M.post_t a)
-      (cs : cond_sol true (post x) pre)
-  : M.tree_cond (M.Tret a x) pre post
-  =
-    M.TCret #a #x pre post (cond_sol_all_to_equiv cs)
-
+[@@ __tac_helper__]
+private
 let __defer_post_unification
       (#a : Type) (#t : M.prog_tree a) (#pre : M.pre_t) (#post0 : M.post_t a)
       (post1 : M.post_t a)
@@ -486,89 +534,315 @@ let __defer_post_unification
   = cd
 
 
-let build_TCspec (post : bool) : Tac unit
+/// While building the [M.tree_cond], we also want to build the associated [M.shape_tree].
+/// This is done by extracting a [pre_shape_tree]. At the end, [build_prog_cond] quotes the [pre_shape_tree],
+/// converts it to a [M.shape_tree] (by using an effective test, [shape_tree_of_pre]) and check that it matches
+/// the built [M.tree_cond] (again with an effective test, [M.tree_cond_has_shape]).
+
+let tc_extract_nat () : Tac nat =
+  norm_cond_sol ();
+  extract_nat_tac ()
+
+[@@ __tac_helper__]
+private
+let __extract_perm (#n : nat) (f : Perm.perm_f n) : Type
+  = extract_term #(list int) (Ll.initi 0 n f)
+
+let tc_extract_perm (n : nat) : Tac (list int) =
+  norm_cond_sol ();
+  extract_term_tac (unquote #(list int))
+
+type pre_shape_tree : (pre_n : int) -> (post_n : int) -> Type =
+  | PSspec  : (pre_n : int) -> (post_n : int) -> (frame_n : int) ->
+              (p0 : list int) -> (p1 : list int) ->
+              pre_shape_tree (pre_n + frame_n) (post_n + frame_n)
+  | PSret   : (n : int) -> (p : list int) ->
+              pre_shape_tree n n
+  | PSbind  : (pre_n : int) -> (itm_n : int) -> (post_n : int) ->
+              (f : pre_shape_tree pre_n itm_n) -> (g : pre_shape_tree itm_n post_n) ->
+              pre_shape_tree pre_n post_n
+  | PSbindP : (pre_n : int) -> (post_n : int) ->
+              (g : pre_shape_tree pre_n post_n) ->
+              pre_shape_tree pre_n post_n
+
+type shape_tree_t = (pre_n : nat & post_n : nat & pre_shape_tree pre_n post_n)
+
+let rec shape_tree_of_pre (#pre_n : nat) (#post_n : nat) (ps : pre_shape_tree pre_n post_n)
+  : Tot (option (M.shape_tree pre_n post_n)) (decreases ps)
+  = match ps with
+  | PSspec pre_n post_n frame_n p0 p1 ->
+           if pre_n >= 0 && post_n >= 0 && frame_n >= 0
+           then match Perm.perm_f_list_checked p0, Perm.perm_f_list_checked p1 with
+           | Some p0, Some p1 -> Some (M.Sspec pre_n post_n frame_n p0 p1)
+           | _ -> None
+           else None
+  | PSret n p ->
+          (match Perm.perm_f_list_checked p with
+          | Some p -> Some (M.Sret n p)
+          | _ -> None)
+  | PSbind pre_n itm_n post_n f g ->
+          if itm_n >= 0
+          then match shape_tree_of_pre f, shape_tree_of_pre g with
+          | Some f, Some g -> Some (M.Sbind pre_n itm_n post_n f g)
+          | _ -> None
+          else None
+  | PSbindP pre_n post_n g ->
+          (match shape_tree_of_pre g with
+          | Some g -> Some (M.SbindP pre_n post_n g)
+          | _ -> None)
+
+
+/// The following tactics solve goals of the form [M.tree_cond t pre t_post] where [t_post] is a concrete term if
+/// the boolean parameter [post] is set and an uvar otherwise.
+/// The resolution is done by solving some [cond_sol] problems. By branching on the [post] parameter, one can
+/// ensure that those problems are fully instantiated. That is we use different building functions depending on
+/// whether the post-condition is known ('_p' (post) functions like [__build_TCspec_p]) or has to be
+/// inferred ('_u' (uvar) functions like [__build_TCspec_u]).
+
+[@@ __tac_helper__]
+private
+let __build_TCspec_u
+      (#a : Type) (#pre : M.pre_t) (#post : M.post_t a) (#req : M.req_t pre) (#ens : M.ens_t pre a post)
+      (#pre' : M.pre_t)
+      (cs0 : cond_sol false pre pre')
+
+      (pre_n   : extract_term (L.length pre))
+      (post_n  : (x : a) -> extract_term (L.length (post x)))
+      (frame_n : extract_term (L.length (cond_sol_unmatched cs0)))
+      (p0 : __extract_perm (cond_sol_to_equiv cs0))
+
+  : M.tree_cond (M.Tspec a pre post req ens) pre' (fun (x : a) -> L.(post x @ cond_sol_unmatched_v cs0))
+  =
+    let frame = cond_sol_unmatched_v cs0 in
+    M.TCspec pre' (fun x -> L.(post x @ frame)) frame
+             (serialize_perm (cond_sol_to_equiv cs0))
+             (fun x -> Perm.id_n (len L.(post x @ frame)))
+
+[@@ __tac_helper__]
+private
+let __build_TCspec_p
+      (#a : Type) (#pre : M.pre_t) (#post : M.post_t a) (#req : M.req_t pre) (#ens : M.ens_t pre a post)
+      (#pre' : M.pre_t) (#post' : M.post_t a)
+      (cs0 : cond_sol false pre pre')
+      (cs1 : (x : a) -> cond_sol true (post' x) L.(post x @ cond_sol_unmatched_v cs0))
+
+      (pre_n   : extract_term (L.length pre))
+      (post_n  : (x : a) -> extract_term (L.length (post x)))
+      (frame_n : extract_term (L.length (cond_sol_unmatched cs0)))
+      (p0 : __extract_perm (cond_sol_to_equiv cs0))
+      (p1 : (x : a) -> __extract_perm (cond_sol_all_to_equiv (cs1 x)))
+
+  : M.tree_cond (M.Tspec a pre post req ens) pre' post'
+  =
+    M.TCspec pre' post' (cond_sol_unmatched_v cs0)
+             (serialize_perm (cond_sol_to_equiv cs0))
+             (fun x -> serialize_perm (cond_sol_all_to_equiv (cs1 x)))
+
+
+[@@ __tac_helper__]
+private
+let __build_TCret_u
+      (#a : Type) (#x : a)
+      (#pre : M.pre_t)
+      (n : extract_term (L.length pre))
+  : M.tree_cond (M.Tret a x) pre (fun _ -> pre)
+  =
+    M.TCret pre (fun _ -> pre) (Perm.id_n (len pre))
+
+[@@ __tac_helper__]
+private
+let __build_TCret_p
+      (#a : Type) (#x : a)
+      (#pre : M.pre_t) (#post : M.post_t a)
+      (cs : cond_sol true (post x) pre)
+      (n : extract_term (L.length pre))
+      (p : __extract_perm (cond_sol_all_to_equiv cs))
+  : M.tree_cond (M.Tret a x) pre post
+  =
+    M.TCret #a #x pre post (serialize_perm (cond_sol_all_to_equiv cs))
+
+
+let build_TCspec (post : bool) : Tac shape_tree_t
   = if post then begin
-      apply_raw (`(__build_TCspec_p));
+      apply_raw (`__build_TCspec_p);
       build_cond_sol false;
       norm_cond_sol ();
       let x = intro () in
       build_cond_sol true
     end else begin
-      // FIXME : why apply_raw shelves sl ?
-      let sl = fresh_uvar None in
-      apply_raw (`(__build_TCspec_u (`#sl)));
-      unshelve sl;
+      // FIXME : why apply_raw shelves cs0 ?
+      let cs0 = fresh_uvar None in
+      apply_raw (`(__build_TCspec_u (`#cs0)));
+      unshelve cs0;
       build_cond_sol false
-    end
+    end;
 
-let build_TCret (post : bool) : Tac unit
+    let pre_n   = tc_extract_nat () in
+    let post_n  = let _ = intro () in tc_extract_nat () in
+    let frame_n = tc_extract_nat () in
+    let p0 = tc_extract_perm (pre_n + frame_n)
+    in let p1 : list int =
+      if post then let _ = intro () in tc_extract_perm (post_n + frame_n)
+      else Ll.initi 0 (post_n + frame_n) id
+    in
+    (|pre_n + frame_n, post_n + frame_n, PSspec pre_n post_n frame_n p0 p1|)
+
+let build_TCret (post : bool) : Tac shape_tree_t
   = if post then begin
        apply_raw (`__build_TCret_p);
        build_cond_sol true
     end else
-      apply_raw (`__build_TCret_u)
+      apply_raw (`__build_TCret_u);
 
-let rec build_TCbind (post : bool) : Tac unit
+    let n = tc_extract_nat () in
+    let p : list int =
+      if post then tc_extract_perm n
+      else Ll.initi 0 n id
+    in
+    (|n, n, PSret n p|)
+
+let rec build_TCbind (post : bool) : Tac shape_tree_t
   = apply (`M.TCbind);
-    // f
-    build_tree_cond false;
+    let (|pre_f, post_f, s_f|) = build_tree_cond false in
     let x = intro () in
-    norm_cond_sol ();
-    // g
-    if post then
-      build_tree_cond true
+    let (|pre_g, post_g, s_g|) = build_tree_cond post  in
+
+    if post_f <> pre_g then cs_raise (fun f -> fail (f (Fail_shape_unification post_f pre_g)));
+    (|pre_f, post_g, PSbind pre_f post_f post_g s_f s_g|)
+
+and build_TCbindP (post : bool) : Tac shape_tree_t
+  = apply (`M.TCbindP);
+    let x = intro () in
+    let (|pre_g, post_g, s_g|) = build_tree_cond post in
+    (|pre_g, post_g, PSbindP pre_g post_g s_g|)
+
+and build_tree_cond (post : bool) : Tac shape_tree_t
+  =
+    let build_tac : bool -> Tac shape_tree_t =
+      let goal = cur_goal () in
+      let args = (collect_app goal)._2 in
+      if L.length args <> 4
+      then cs_raise (fun f -> fail (f (Fail_goal_shape GShape_tree_cond goal)))
+      else let hd = (collect_app (L.index args 1)._1)._1 in
+      match inspect hd with
+      | Tv_FVar fv ->
+          // TODO? better solution to match
+          let nd = inspect_fv fv in
+          if Nil? nd then cs_raise (fun f -> fail (f (Fail_goal_shape GShape_tree_cond goal)));
+          begin match L.last nd with
+          | "Tspec"  -> build_TCspec
+          | "Tret"   -> build_TCret 
+          | "Tbind"  -> build_TCbind
+          | "TbindP" -> build_TCbindP
+          | _ -> cs_raise (fun f -> fail (f (Fail_goal_shape GShape_tree_cond goal)))
+          end
+      | _ -> cs_raise (fun f -> fail (f (Fail_goal_shape GShape_tree_cond goal)))
+    in
+    if post
+    then build_tac true
     else begin
-      // If post is false, the post is an uvar [post0] independent of [x].
-      // The inferred post of [g] can depend (but should not) on [x].
-      // Since we may need to normalize the inferred post in order to see that it does not depends on [x],
-      // we introduce a fresh uvar [post1] that can depends on [x] and then prove that we can chose it for
-      // the post [post0] of the bind.
+      // If post is false, the post is an uvar [post0] that may be independent of some bound variables the current
+      // [M.prog_tree] and pre can depend on.
+      // If we try to build directly a [tree_cond_sol] for [post0], the unification can fail since we need
+      // to normalize the inferred post in order to see the variables it depends on.
+      // Hence we introduce a fresh uvar [post1] for the inferred post. [post1] can depend on all the variables
+      // in scope but should (in a correct program) only depends on the variables in scope for [post0].
+      // We then normalize [post1] and try to assign the result to [post0].
       let post1 = fresh_uvar None in
+      // Changes the goal [tree_cond_sol t pre ?post0] into [tree_cond_sol t pre ?post1] and [?post0 == ?post1]
       apply_raw (`(__defer_post_unification (`#post1)));
-      build_tree_cond false;
-      trefl () // [post0] <- [post1]
+      // Solves [tree_cond_sol t pre post1]
+      let shp = build_tac false in
+      // [?post1] is now inferred as [post1] and we are presented with a goal [?post0 == post1].
+      // We normalize [post1] and assign the result to [?post0].
+      norm_cond_sol ();
+      cs_try trefl (fun f -> fail (f Fail_post_unification));
+
+      shp
     end
 
-and build_tree_cond (post : bool) : Tac unit
-  =
-    let goal = cur_goal () in
-    let args = (collect_app goal)._2 in
-    if L.length args < 4
-    then fail "goal is not a tree_cond"
-    else let hd = (collect_app (L.index args 1)._1)._1 in
-    match inspect hd with
-    | Tv_FVar fv ->
-        // TODO? better solution to match
-        let nd = inspect_fv fv in
-        if Nil? nd then fail "empty fv";
-        begin match L.last nd with
-        | "Tspec"  -> build_TCspec post
-        | "Tret"   -> build_TCret  post
-        | "Tbind"  -> build_TCbind post
-        | "TbindP" -> fail "TODO"
-        | _ -> fail ("build_tree_cond: head is "^(implode_qn nd))
-        end
-    | _ -> fail ("build_tree_cond: head is "^term_to_string hd)
+
+[@@ __tac_helper__]
+private
+let __build_prog_cond
+      (#a : Type) (#t : M.prog_tree a) (#pre : M.pre_t) (#post : M.post_t a)
+      (tc0 : M.tree_cond t pre post)
+      (#tc : M.tree_cond t pre post) (_ : squash (tc == tc0)) // allows to normalize tc
+      (#pre_n : int) (#post_n : int) (ps : pre_shape_tree pre_n post_n)
+      (_ : squash (pre_n >= 0 /\ post_n >= 0 /\ pre_n == len pre))
+      (#s : M.shape_tree pre_n post_n) (_ : squash (Some s == shape_tree_of_pre ps))
+      (_ : M.tree_cond_has_shape tc s)
+  : M.prog_cond t pre post
+  = (|tc, {M.post_len = post_n; shp = s}|)
+
+let intro_l_True : l_True = ()
+let intro_squash_l_True : squash (l_True) = ()
+
+/// This is the front-end tactics. It solves a goal of the form [M.prog_cond t pre post].
+let build_prog_cond () : Tac unit
+  = 
+    let tc0   = fresh_uvar None in
+    let tc_eq = fresh_uvar None in
+    let ushp  = fresh_uvar None in
+    apply (`(__build_prog_cond (`#tc0) (`#tc_eq) (`#ushp)));
+    // [M.tree_cond t pre post]
+    unshelve tc0;
+    let (|pre_n, post_n, shp|) = build_tree_cond true in
+    // tc <- tc0
+    unshelve tc_eq;
+    norm_cond_sol ();
+    trefl ();
+    // shp
+    unshelve ushp;
+    exact (quote shp);
+    // some checks
+    norm [delta_only [`%L.length; `%len]; iota; zeta; primops; simplify];
+    exact (`intro_squash_l_True);
+    // [shape_tree_of_pre]
+    norm [delta_only [`%shape_tree_of_pre;
+                      `%Perm.perm_f_list_checked; `%Perm.check_list_injective;
+                      `%L.length; `%L.hd; `%L.tl; `%L.tail; `%Ll.initi; `%L.index; `%L.list_ref; `%Ll.set
+                     ];
+          iota; zeta; primops];
+    trefl ();
+    // [M.tree_cond_has_shape tc shp]
+    norm [delta_only [`%M.tree_cond_has_shape; `%Perm.perm_f_to_list; `%Perm.mk_perm_f; `%Perm.mk_perm_f;
+                      `%Perm.perm_f_eq; `%Perm.perm_f_of_list; `%Perm.id_n;
+                      `%L.length; `%L.hd; `%L.tl; `%L.tail; `%L.index; `%Ll.initi; `%Ll.list_eq;
+                      `%U.cast];
+          delta_qualifier ["unfold"];
+          iota; zeta; primops; simplify];
+    exact (`intro_l_True)
+
+
+(*** Test *)
+
+open Steel.Effect.Common
+
+unfold
+let specT (a : Type) (pre : M.pre_t) (post : M.post_t a) : M.prog_tree a
+  = M.Tspec a pre post (fun _ -> True) (fun _ _ _ -> True)
+
+let norm_test () : Tac unit = norm [delta_qualifier ["unfold"]]
 
 
 let _test_TCspec_u (v0 v1 : vprop') : squash True =
   _ by (let post' = fresh_uvar (Some (`(M.post_t int))) in
-        let _,() =
-          build (`(M.tree_cond
-            (M.Tspec int [(`@v0)] (fun _ -> [(`@v1)]) (fun _ -> True) (fun _ _ _ -> True))
-            [(`@v0)] (`#post')))
-          (fun () -> build_TCspec false)
+        let _ =
+          build (`(M.tree_cond (specT int [(`@v0)] (fun _ -> [(`@v1)]))
+                               [(`@v0)] (`#post')))
+          (fun () -> norm_test (); build_TCspec false)
         in ())
 
 let _test_TCspec_p (v0 v1 v2 : vprop') (vx : int -> vprop')
-  : M.tree_cond (M.Tspec int [v0; v1] (fun x -> [v0; vx x]) (fun _ -> True) (fun _ _ _ -> True))
+  : M.tree_cond (specT int [v0; v1] (fun x -> [v0; vx x]))
                 ([v0; v1; v2]) (fun x -> [v2; vx x; v0])
-  = _ by (build_TCspec true)
+  = _ by (norm_test (); let _ = build_TCspec true in ())
 
 
 let _test_TCret_u (v0 v1 : vprop') : squash True =
   _ by (let post' = fresh_uvar (Some (`(M.post_t int))) in
-        let _,() =
+        let _,_ =
           build (`(M.tree_cond (M.Tret int 42) [(`@v0); (`@v1)] (`#post')))
           (fun () -> build_TCret false)
         in ())
@@ -576,46 +850,131 @@ let _test_TCret_u (v0 v1 : vprop') : squash True =
 let _test_TCret_p (v0 : vprop') (vx0 vx1 : int -> vprop')
   : M.tree_cond (M.Tret int 42)
                 ([v0; vx0 42; vx1 42]) (fun x -> [v0; vx1 x; vx0 42])
-  = _ by (build_TCret true)
+  = _ by (let _ = build_TCret true in ())
 
 
 let _test_TCbind_u (v0 v1 : vprop') (vx0 : int -> vprop') : squash True =
   _ by (let post' = fresh_uvar (Some (`(M.post_t int))) in
         let _,() =
           build (`(M.tree_cond
-            (M.Tbind int int (M.Tspec int []          (fun x -> [(`@vx0) x]) (fun _ -> True) (fun _ _ _ -> True))
-                   (fun x -> M.Tspec int [(`@vx0) x] (fun _ -> [(`@v1)])    (fun _ -> True) (fun _ _ _ -> True)))
+            (M.Tbind int int (specT int []          (fun x -> [(`@vx0) x]))
+                   (fun x -> specT int [(`@vx0) x] (fun _ -> [(`@v1)])))
             [(`@v0)] (`#post')))
           (fun () ->
+            norm_test ();
             apply (`M.TCbind);
-            build_TCspec false;
+            let _ = build_TCspec false in
             let x = intro () in
             norm_cond_sol ();
             let post1 = fresh_uvar None in
             apply_raw (`(__defer_post_unification (`#post1)));
-            build_TCspec false;
-            norm_cond_sol ();
-            trefl ()
+            let _ = build_TCspec false in
+            norm_cond_sol (); trefl ()
           )
         in ())
 
 let _test_TCbind_p (v0 v1 : vprop') (vx0 vx1 : int -> vprop')
   : M.tree_cond
-        (M.Tbind int int (M.Tspec int []      (fun x -> [vx0 x])     (fun _ -> True) (fun _ _ _ -> True))
-               (fun x -> M.Tspec int [vx0 x] (fun y -> [v1; vx1 y]) (fun _ -> True) (fun _ _ _ -> True)))
+        (M.Tbind int int (specT int []      (fun x -> [vx0 x])    )
+               (fun x -> specT int [vx0 x] (fun y -> [v1; vx1 y])))
             [v0] (fun y -> [v0; vx1 y; v1])
   = _ by (
+    norm_test ();
     apply (`M.TCbind);
-    build_TCspec false;
+    let _ = build_TCspec false in
     let x = intro () in
     norm_cond_sol ();
-    build_TCspec true
+    let _ = build_TCspec true in
+    ()
+  )
+
+
+let _test_TCbindP_u (v0 v1 : vprop') (vx0 : int -> vprop') (wp : pure_wp int) (f : unit -> PURE int wp) : squash True =
+  _ by (let post' = fresh_uvar (Some (`(M.post_t int))) in
+        let _,() =
+          build (`(M.tree_cond
+            (M.TbindP int int (`@wp) (`@f)
+                    (fun x -> specT int [(`@v0)] (fun y -> [(`@vx0) y])))
+            [(`@v0); (`@v1)] (`#post')))
+          (fun () ->
+            norm_test ();
+            apply (`M.TCbindP);
+            let x = intro () in
+            let post1 = fresh_uvar None in
+            apply_raw (`(__defer_post_unification (`#post1)));
+            let _ = build_TCspec false in
+            norm_cond_sol (); trefl ()
+          )
+        in ())
+
+let _test_TCbindP_p (v0 v1 : vprop') (vx0 : int -> vprop') (wp : pure_wp int) (f : unit -> PURE int wp)
+  : M.tree_cond
+        (M.TbindP int int wp f
+                (fun x -> specT int [v0] (fun y -> [vx0 y])))
+            [v0; v1] (fun y -> [v1; vx0 y])
+  = _ by (
+    norm_test ();
+    apply (`M.TCbindP);
+    let x = intro () in
+    let _ = build_TCspec true in ()
   )
 
 
 let _test_build_tree_cond_0 (v0 v1 : vprop') (vx0 vx1 : int -> vprop')
   : M.tree_cond
-        (M.Tbind int int (M.Tspec int []      (fun x -> [vx0 x])     (fun _ -> True) (fun _ _ _ -> True))
-               (fun x -> M.Tspec int [vx0 x] (fun y -> [v1; vx1 y]) (fun _ -> True) (fun _ _ _ -> True)))
+        (M.Tbind int int (specT int []      (fun x -> [vx0 x]))
+               (fun x -> specT int [vx0 x] (fun y -> [v1; vx1 y])))
             [v0] (fun y -> [v0; vx1 y; v1])
-  = _ by (build_tree_cond true)
+  = _ by (norm_test (); let shp = build_tree_cond true in _)
+
+let _test_build_prog_cond_0 (v0 v1 : vprop') (vx0 vx1 : int -> vprop')
+  : M.prog_cond
+        (M.Tbind int int (specT int []      (fun x -> [vx0 x]))
+               (fun x -> specT int [vx0 x] (fun y -> [v1; vx1 y])))
+        [v0] (fun y -> [v0; vx1 y; v1])
+  = _ by (norm_test (); build_prog_cond ())
+
+let _ = fun v0 v1 vx0 vx1 ->
+  assert (U.print_util (_test_build_prog_cond_0 v0 v1 vx0 vx1))
+      by (norm [delta_only [`%_test_build_prog_cond_0]];
+          norm_test ();
+          norm_cond_sol ();
+          dump "print")
+
+// This example fails because the resolution of the innermost [M.Tret] has to infer its post. In this case the
+// inferred post is simply the current vprops, ignoring the returned value (i.e. [fun _ -> pre] in [__build_TCret_u]).
+// But at this point pre is [vx0 x] where [x] is bound, the inferred post is thus [fun _ -> [vx0 x]] which
+// depends on [x].
+[@@expect_failure [228]]
+let _test_build_tree_cond_1 (vx0 : int -> vprop')
+  : M.tree_cond
+        (M.Tbind int int
+            (M.Tbind int int (specT int [] (fun x -> [vx0 x])) (fun x -> M.Tret int x))
+            (fun x -> M.Tret int x))
+        [] (fun x -> [vx0 x])
+  = _ by (norm_test (); let _ = build_tree_cond true in ())
+
+// This example works because the resolution of [M.Tret] is given the expected post (the post of the whole
+// program), [fun x' -> [vx0 x']].
+let _test_build_tree_cond_2 (vx0 : int -> vprop')
+  : M.tree_cond
+        (M.Tbind int int (specT int [] (fun x -> [vx0 x])) (fun x -> M.Tret int x))
+        [] (fun x -> [vx0 x])
+  = _ by (norm_test (); let _ = build_tree_cond true in ())
+
+// This example fails because we cannot find a [v0] in the pre.
+[@@expect_failure [228]]
+let _test_build_tree_cond_3 (v0 : vprop')
+  : M.tree_cond
+        (specT int [v0] (fun _ -> []))
+        [] (fun _ -> [])
+  = _ by (norm_test (); let _ = build_tree_cond true in ())
+
+// This example fails because we obtain [fun _ -> [v0]] as post which is not unifiable with the expected post
+// [fun _ -> []]
+[@@expect_failure [228]]
+let _test_build_tree_cond_4 (v0 : vprop')
+  : M.tree_cond
+        (specT int [] (fun _ -> [v0]))
+        [] (fun _ -> [])
+  = _ by (norm_test (); let _ = build_tree_cond true in ())
