pure/Learn.Tactics.Util.fst
@@ -5,6 +5,9 @@ module L = FStar.List.Pure
 open FStar.Tactics
 
 
+irreducible let __tac_helper__ : unit = ()
+
+[@@ __tac_helper__]
 private
 let __pose (goal:Type) (#t:Type) (x : t) (f : t -> goal) : goal = f x
 
@@ -12,6 +15,7 @@ let pose (t : term) : Tac binder =
   apply (`__pose (`#(cur_goal ())) (`#t));
   intro ()
 
+[@@ __tac_helper__]
 private
 let __build (goal:Type) (t : Type) (x : t) (f : t -> goal) : goal = f x
 
@@ -35,3 +39,32 @@ let rec repeatb (#a : Type) (t : unit -> Tac (option a)) : Tac (list a) =
   match t () with
   | Some x -> x :: repeatb t
   | None   -> []
+
+
+let extract_term (#a : Type) (x : a) : Type = unit
+
+let __extract_term_end (#a : Type) (x : a) : extract_term x = ()
+
+/// On a goal [extract_term t], this tactics returns [f t] and solves the goal
+let extract_term_tac (#a : Type) (f : term -> Tac a) : Tac a
+  = let goal = cur_goal () in
+    let view = inspect goal in
+    match view with
+    | Tv_App _ (t, Q_Explicit) ->
+             let res = f t in // f is ran before solving the goal
+             apply (`__extract_term_end);
+             res
+    | _ -> fail ("failed to extract term from "^term_to_string goal)
+
+/// On a goal [extract_term n], this tactics returns the integer [n] and solves the goal
+let extract_int_tac () : Tac int
+  = extract_term_tac (fun t ->
+    match inspect t with
+    | Tv_Const (C_Int n) -> n
+    | _ -> fail ("failed to extract int from "^term_to_string t))
+
+/// On a goal [extract_term n], this tactics returns the natural [n] and solves the goal
+let extract_nat_tac () : Tac nat
+  = let n = extract_int_tac () in
+    if n < 0 then fail ("extracted int "^string_of_int n^" < 0");
+    n
